fix with_hide_buffer `modifies` bounds, derive some instances

src/QUIC.Secret.Buffer.fst
@@ -38,18 +38,7 @@ let with_buffer_hide #t b from to h0 lin lout x1 x2 x3 x4 x5 x6 post f =
   let br = B.offset b to in
   f (Ghost.hide (B.loc_buffer b)) bl bs br
 
-let with_buffer_hide_weak_modifies #t b from to h0 lin lout ml ms mr post f =
-  let bl = B.sub b 0ul from in
-  let bs = B.sub b from (to `U32.sub` from) in
-  let br = B.offset b to in
-  f (Ghost.hide (B.loc_buffer b)) bl bs br
-
 let with_buffer_hide_from #t b from h0 lin lout x1 x2 x3 x4 post f =
-  let bl = B.sub b 0ul from in
-  let bs = B.offset b from in
-  f (Ghost.hide (B.loc_buffer b)) bl bs
-
-let with_buffer_hide_from_weak_modifies #t b from h0 lin lout ml ms post f =
   let bl = B.sub b 0ul from in
   let bs = B.offset b from in
   f (Ghost.hide (B.loc_buffer b)) bl bs
